src/zksync_verifier.ec
@@ -6,26 +6,52 @@ require import Utils.
 op p = W256.of_int 21888242871839275222246405745257275088696311157297823662689037894645226208583.
 
 module Test = {
-    proc pointNegate(point : uint256) : unit = {
-      var _1, _2, _3, pY, tmp166, tmp167, tmp168, _6, _7;
-      _1 <- W256.of_int 32;
-      _2 <- point + _1;
-      tmp166 <@ Primops.mload(_2);
-      pY <- tmp166;
-      tmp167 <- pY;
-      if (tmp167 = W256.of_int 0)
+
+    proc usr_revertWithMessage(usr_len : uint256, usr_reason : uint256): unit = {
+    var _1, _2, _3, _4, _5, _6, _7;
+    _1 <- (shl (W256.of_int 229) (W256.of_int 4594637));
+    _2 <- (W256.of_int 0);
+    Primops.mstore(_2, _1);
+    _3 <- (W256.of_int 32);
+    _4 <- (W256.of_int 4);
+    Primops.mstore(_4, _3);
+    _5 <- (W256.of_int 36);
+    Primops.mstore(_5, usr_len);
+    _6 <- (W256.of_int 68);
+    Primops.mstore(_6, usr_reason);
+    _7 <- (W256.of_int 100);
+    Primops.revert(_2, _7);
+    }
+
+  proc usr_pointNegate(usr_point : uint256): unit = {
+    var _1, _2, usr_pY, tmp88, tmp89, _3, tmp90, _4, _5, tmp91, _6, _7;
+    _1 <- (W256.of_int 32);
+    _2 <- (usr_point + _1);
+    tmp88 <@ Primops.mload(_2);
+    usr_pY <- tmp88;
+    tmp89 <- usr_pY;
+    if ((tmp89 = (W256.of_int 0)))
       {
-        tmp168 <@ Primops.mload(point);
-        _3 <- tmp168;
-        if (_3 = W256.of_int 0)
+      tmp90 <@ Primops.mload(usr_point);
+      _3 <- tmp90;
+      if (bool_of_uint256 _3)
         {
-          Primops.revert();
+        _4 <- STRING (*pointNegate: invalid point*);
+        _5 <- (W256.of_int 26);
+        tmp91 <@ usr_revertWithMessage(_5, _4);
+
         }
-      } else {
-          _6 <- W256.of_int 21888242871839275222246405745257275088696311157297823662689037894645226208583;
-          _7 <- _6 - pY;
-          Primops.mstore(_2, _7);
+
+
       }
+
+    else {
+      _6 <- (W256.of_int 21888242871839275222246405745257275088696311157297823662689037894645226208583);
+      _7 <- (_6 - usr_pY);
+      Primops.mstore(_2, _7);
+
+      }
+
     }
 
     proc writeReadTest(address: uint256, value: uint256): uint256 = {
@@ -54,10 +80,10 @@ proof.
   progress.
   apply ConcretePrimops.apply_mstore_mload_same.
 qed.
-      
+
 lemma pointNegate_correctness :
     forall (x y point_addr : uint256),
-hoare [ Test.pointNegate :
+hoare [ Test.usr_pointNegate :
     arg = point_addr /\
     (x <> W256.zero \/ y <> W256.zero) /\
         Primops.memory.[point_addr] = x /\
@@ -73,7 +99,7 @@ hoare [ Test.pointNegate :
     progress.
     proc.
     simplify.
-    inline Primops.mload Primops.mstore Primops.revert.
+    inline Test.usr_revertWithMessage Primops.mload Primops.mstore Primops.revert.
     wp.
     skip.
     progress.
