src/UInt256.ec
@@ -6,3 +6,6 @@ type uint256 = W256.t.
 
 abbrev (%%) (m d : uint256) = W256.\umod m d.
 abbrev (<)  (a b : uint256) = W256.\ult a b.
+
+op bool_of_uint256 (x : uint256) : bool = x = W256.one.
+op eq_uint256(a : uint256, b : uint256) : uint256  = if a = b then W256.one else W256.zero.
